Renaming in rel.v

lib/rel.v
@@ -18,41 +18,52 @@ From SimpleIO Require Import
 From advent.lib Require Import
      io.
 
-Record io_state := Mk_io_state {
-  input : list Z;
-  output : list Z;
+(* State [s -> (s * a)] as a relation. *)
+Definition state_rel (S : Type) (A : Type) : Type :=
+  S -> S -> A -> Prop.
+
+Record io_state (I O : Type) := Mk_io_state {
+  input : list I;
+  output : list O;
 }.
 
-Definition initial (i : list Z) : io_state := Mk_io_state i [].
+Arguments Mk_io_state {I O} _ _.
+Arguments input {I O} _.
+Arguments output {I O} _.
 
-Definition drop_input (r : io_state) : io_state :=
+Definition initial {I O : Type} (i : list I) : io_state I O :=
+  Mk_io_state i [].
+
+Definition drop_input {I O : Type} (r : io_state I O) : io_state I O :=
   let '(Mk_io_state i o) := r in
   Mk_io_state (tl i) o.
 
-Definition push_output (z : Z) (r : io_state) : io_state :=
+Definition push_output {I O : Type}
+           (z : O) (r : io_state I O) : io_state I O :=
   let '(Mk_io_state i o) := r in
   Mk_io_state i (o ++ [z]).
 
-(* State [s -> (s * a)] as a relation. *)
-Definition state_rel (s : Type) (a : Type) : Type :=
-  s -> s -> a -> Prop.
+Definition io_rel (I O : Type) : Type -> Type :=
+  state_rel (io_state I O).
 
-Definition io_rel : Type -> Type := state_rel io_state.
+Definition rel_spec (I O : Type) :
+  io_rel I O unit -> list I -> list O -> Prop :=
+  fun x i o =>
+    exists s,
+      x (initial i) s tt /\
+      output s = o.
 
-Definition rel_spec : io_rel unit -> io_state -> io_state -> Prop :=
-  fun x i o => x i o tt.
-
-Instance Monad_state_rel s : Monad (state_rel s) := {
+Instance Monad_state_rel (S : Type) : Monad (state_rel S) := {
   ret _ x := fun s1 s2 x' => s2 = s1 /\ x' = x;
   bind _ _ m k := fun s1 s3 y =>
     exists x s2, m s1 s2 x /\ k x s2 s3 y
 }.
 
-Instance MonadError_state_rel s : MonadError (state_rel s) := {
+Instance MonadError_state_rel (S : Type) : MonadError (state_rel S) := {
   error _ _ := fun _ _ _ => False
 }.
 
-Instance MonadIZ_io_rel : MonadI Z io_rel := {
+Instance MonadI_io_rel (I O : Type) : MonadI I (io_rel I O) := {
   read := fun s1 s2 x' =>
     (exists z,
       input s1 = z :: input s2 /\
@@ -61,42 +72,41 @@ Instance MonadIZ_io_rel : MonadI Z io_rel := {
     (s2 = s1 /\ x' = None);
 }.
 
-Instance MonadOZ_io_rel : MonadO Z io_rel := {
+Instance MonadO_io_rel (I O : Type) : MonadO O (io_rel I O) := {
   print z := fun s1 s2 x' =>
     s2 = push_output z s1 /\
     x' = tt
 }.
 
-Definition incl_rel_1 {a b s : Type}
-           (r1 r2 : a -> state_rel s b) :=
-  forall x z1 z2 y,
-    r1 x z1 z2 y -> r2 x z1 z2 y.
+Definition incl_rel {S A : Type} (r1 r2 : state_rel S A) :=
+  forall s1 s2 a, r1 s1 s2 a -> r2 s1 s2 a.
 
-Lemma incl_rel_1_refl {a b s : Type} (r : a -> state_rel s b) :
+Definition incl_rel_1 {S A B : Type}
+           (r1 r2 : A -> state_rel S B) :=
+  forall x, incl_rel (r1 x) (r2 x).
+
+Lemma incl_rel_1_refl {S A B : Type} (r : A -> state_rel S B) :
   incl_rel_1 r r.
 Proof.
   intros x z1 z2 y; auto.
 Qed.
 
-Inductive lfp_rel {a b : Type} {s : Type}
-          (gf : (a -> state_rel s b) -> (a -> state_rel s b))
-          (x : a)
-          (z1 : s)
-          (z2 : s)
-          (y : b) : Prop :=
+Inductive lfp_rel {S A B : Type}
+          (gf : (A -> state_rel S B) -> (A -> state_rel S B))
+          (a : A) (s1 s2 : S) (b : B) : Prop :=
 | LFP
-    (P : a -> state_rel s b)
+    (P : A -> state_rel S B)
     (P_ind : incl_rel_1 P (lfp_rel gf))
-    (P_holds : gf P x z1 z2 y).
+    (P_holds : gf P a s1 s2 b).
 
-Definition monotonic_rel {a b : Type} {s : Type}
-           (gf : (a -> state_rel s b) -> (a -> state_rel s b)) :=
+Definition monotonic_rel {S A B : Type}
+           (gf : (A -> state_rel S B) -> (A -> state_rel S B)) :=
   forall r1 r2,
     incl_rel_1 r1 r2 ->
     incl_rel_1 (gf r1) (gf r2).
 
-Lemma lfp_rel_unfold {a b : Type} {s : Type}
-      (gf : (a -> state_rel s b) -> (a -> state_rel s b))
+Lemma lfp_rel_unfold {S A B : Type}
+      (gf : (A -> state_rel S B) -> (A -> state_rel S B))
       (mon_gf : monotonic_rel gf) :
   incl_rel_1 (lfp_rel gf) (gf (lfp_rel gf)).
 Proof.
@@ -106,8 +116,8 @@ Proof.
   apply P_holds.
 Qed.
 
-Lemma lfp_rel_fold {a b s : Type}
-      (gf : (a -> state_rel s b) -> (a -> state_rel s b)) :
+Lemma lfp_rel_fold {S A B : Type}
+      (gf : (A -> state_rel S B) -> (A -> state_rel S B)) :
   incl_rel_1 (gf (lfp_rel gf)) (lfp_rel gf).
 Proof.
   intros x z1 z2 y Hgf.
@@ -116,10 +126,10 @@ Proof.
   auto.
 Qed.
 
-Lemma really_lfp {a b s : Type}
-      (gf : (a -> state_rel s b) -> (a -> state_rel s b))
+Lemma really_lfp {S A B : Type}
+      (gf : (A -> state_rel S B) -> (A -> state_rel S B))
       (mon_gf : monotonic_rel gf)
-      (fp : a -> state_rel s b)
+      (fp : A -> state_rel S B)
       (H_fp : incl_rel_1 (gf fp) fp) :
   incl_rel_1 (lfp_rel gf) fp.
 Proof.
@@ -129,6 +139,6 @@ Proof.
   apply mon_gf with (r1 := P); auto.
 Qed.
 
-Instance MonadFix_state_rel s : MonadFix (state_rel s) := {
+Instance MonadFix_state_rel (S : Type) : MonadFix (state_rel S) := {
   mfix _ _ := lfp_rel
 }.
